PTR.v
@@ -1,4 +1,5 @@
 (*
+  PTR.v
   Pointer Analysis for TAC IR
 *)
 
@@ -9,19 +10,22 @@ Import ListNotations.
 
 Set Implicit Arguments.
 
-Import TAC.
+Require Import IR.
+Require Import SIGS.
 
-Module PointerAnalysis.
+Module PointerAnalysis (TS : TypeSystemSig).
+  Import TAC TS.
 
-  (* ===== Abstract Objects ===== *)
+  (* Abstract Objects *)
   Module AbstractObject.
     Inductive t :=
-    | Location : nat -> nat -> t           (* allocation site: (block, instr) *)
-    | Param    : option string -> t        (* parameter with optional name *)
-    | ImmType  : nat -> t                  (* immutable by type hash *)
-    | ImmConst : ConstV -> t               (* immutable constant value *)
-    | Locals   : t                         (* locals scope *)
-    | Globals  : t.                        (* globals scope *)
+    | Location : nat -> nat -> t
+    | Param    : option string -> t
+    | ImmType  : nat -> t
+    | ImmConst : ConstV -> t
+    | Locals   : t
+    | Globals  : t.
+    
     Definition eq_dec : forall x y : t, {x = y} + {x <> y}.
     Proof.
       decide equality; try apply Nat.eq_dec; try apply String.string_dec.
@@ -31,599 +35,535 @@ Module PointerAnalysis.
     Defined.
   End AbstractObject.
 
-  Module Type TypeSystemSig.
-    Import AbstractObject.
+  (* Core Domains *)
+  Module AODec <: DecidableType.
+    Definition t := AbstractObject.t.
+    Definition eq := @eq t.
+    Definition eq_refl := @eq_refl t.
+    Definition eq_sym := @eq_sym t.
+    Definition eq_trans := @eq_trans t.
+    Definition eq_dec := AbstractObject.eq_dec.
+  End AODec.
 
-    Parameter TypeExpr : Type.
-    Parameter type_bot : TypeExpr.
-    Parameter type_top : TypeExpr.
-    Parameter type_join : TypeExpr -> TypeExpr -> TypeExpr.
-    Parameter type_is_subtype : TypeExpr -> TypeExpr -> bool.
-    Parameter type_is_immutable : TypeExpr -> bool.
+  Module ObjectSet := FSetWeakList.Make(AODec).
+  Module AOMap := FMapWeakList.Make(AODec).
 
-    Record SideEffect := {
-      se_new : bool;
-      se_bound_method : bool;
-      se_update : option TypeExpr;
-      se_update_indices : list nat;
-      se_points_to_args : bool
-    }.
-    Parameter empty_effect : SideEffect.
+  Module FKDec <: DecidableType.
+    Definition t := FieldKey.
+    Definition eq := @eq t.
+    Definition eq_refl := @eq_refl t.
+    Definition eq_sym := @eq_sym t.
+    Definition eq_trans := @eq_trans t.
+    Definition eq_dec : forall x y : t, {x = y} + {x <> y}.
+    Proof. decide equality; try apply Nat.eq_dec; try apply String.string_dec. Defined.
+  End FKDec.
 
-    Parameter literal_type : ConstV -> TypeExpr.
-    Parameter get_type_hash : TypeExpr -> nat.
+  Module FieldMap := FMapWeakList.Make(FKDec).
 
-    Parameter is_overloaded : TypeExpr -> bool.
-    Parameter is_property : TypeExpr -> bool.
-    Parameter is_bound_method : TypeExpr -> bool.
-    Parameter any_new : TypeExpr -> bool.
-    Parameter all_new : TypeExpr -> bool.
-    Parameter get_return : TypeExpr -> TypeExpr.
-    Parameter get_side_effect : TypeExpr -> SideEffect.
+  Definition PointsTo := AOMap.t (FieldMap.t ObjectSet.t).
+  Definition TypeMap  := AOMap.t TypeExpr.
+  Definition DirtyMap := AOMap.t (FieldMap.t bool).
+  Definition StackEnv := StackVar -> ObjectSet.t.
+  Definition ProgramPoint := (nat * nat)%type.
 
-    Parameter subscr : TypeExpr -> string -> TypeExpr.
-    Parameter subscr_literal : TypeExpr -> ConstV -> TypeExpr.
-    Parameter subscr_index : TypeExpr -> nat -> TypeExpr.
+  (* Field Key Helpers *)
+  Definition wildcard    : FieldKey := FKName "*".
+  Definition self_field  : FieldKey := FKName "self".
+  Definition func_field  : FieldKey := FKName "__func__".
+  Definition args_field  : FieldKey := FKName "args".
+  Definition kwargs_field: FieldKey := FKName "kwargs".
 
-    Parameter partial : TypeExpr -> list TypeExpr -> TypeExpr.
-    Parameter get_unop : TypeExpr -> string -> TypeExpr.
-    Parameter partial_binop : TypeExpr -> TypeExpr -> string -> TypeExpr.
+  Definition is_star (k:FieldKey) : bool :=
+    match k with | FKName s => String.eqb s "*" | _ => false end.
 
-    Parameter make_list_constructor : TypeExpr.
-    Parameter make_tuple_constructor : TypeExpr.
-    Parameter make_dict_constructor : TypeExpr.
-    Parameter make_set_constructor : TypeExpr.
-    Parameter make_slice_constructor : TypeExpr.
+  Definition field_matches (k1 k2 : FieldKey) : bool :=
+    if orb (is_star k1) (is_star k2) then true else
+    match k1, k2 with
+    | FKPos n1,  FKPos n2  => Nat.eqb n1 n2
+    | FKName s1, FKName s2 => String.eqb s1 s2
+    | FKBoth n1 s1, FKBoth n2 s2 => Nat.eqb n1 n2 && String.eqb s1 s2
+    | FKPos n,   FKBoth n' _ | FKBoth n' _, FKPos n   => Nat.eqb n n'
+    | FKName s,  FKBoth _ s' | FKBoth _ s', FKName s  => String.eqb s s'
+    | _, _ => false
+    end.
 
-    Parameter type_is_callable : TypeExpr -> bool.
+  (* Empty/Initial Values *)
+  Definition empty_points_to : PointsTo := AOMap.empty _.
+  Definition empty_type_map  : TypeMap  := AOMap.empty _.
+  Definition empty_dirty_map : DirtyMap := AOMap.empty _.
+  Definition empty_stack     : StackEnv := fun _ => ObjectSet.empty.
 
-    (* === New: operator resolution with typed operands === *)
-    Inductive DunderInfo :=
-    | TDUnOp  (op:UnOpTag)  (arg:TypeExpr)
-    | TDBinOp (op:BinOpTag) (lhs rhs:TypeExpr) (mode:Inplace)
-    | TDCmpOp (op:CmpOpTag) (lhs rhs:TypeExpr).
+  (* Helpers for immutables *)
+  Definition immutable_const (c : ConstV) : ObjectSet.t :=
+    ObjectSet.singleton (AbstractObject.ImmConst c).
+  Definition immutable_type (ty : TypeExpr) : ObjectSet.t :=
+    ObjectSet.singleton (AbstractObject.ImmType (get_type_hash ty)).
 
-    Parameter dunder_lookup : DunderInfo -> TypeExpr.
-  End TypeSystemSig.
+  (* Keep FieldMap sparse *)
+  Definition fm_add_nonempty (fm : FieldMap.t ObjectSet.t)
+                             (k : FieldKey) (objs : ObjectSet.t)
+    : FieldMap.t ObjectSet.t :=
+    if ObjectSet.is_empty objs then FieldMap.remove k fm
+    else FieldMap.add k objs fm.
 
-  Module Analysis (TS : TypeSystemSig).
-    Import TS AbstractObject.
+  (* Points-to ops *)
+  Definition points_to_lookup (P : PointsTo) (o : AbstractObject.t) (f : FieldKey) : ObjectSet.t :=
+    match AOMap.find o P with
+    | Some fm =>
+        FieldMap.fold (fun k objs acc =>
+          if orb (field_matches k f) (field_matches f k)
+          then ObjectSet.union acc objs
+          else acc) fm ObjectSet.empty
+    | None => ObjectSet.empty
+    end.
 
-    (* ===== Core Domains ===== *)
-    Module AODec <: DecidableType.
-      Definition t := AbstractObject.t.
-      Definition eq := @eq t.
-      Definition eq_refl := @eq_refl t.
-      Definition eq_sym := @eq_sym t.
-      Definition eq_trans := @eq_trans t.
-      Definition eq_dec := AbstractObject.eq_dec.
-    End AODec.
+  Definition points_to_update (P : PointsTo) (o : AbstractObject.t) (f : FieldKey)
+                              (objs : ObjectSet.t) : PointsTo :=
+    let fm := match AOMap.find o P with
+              | Some fm => fm | None => FieldMap.empty _
+              end in
+    AOMap.add o (fm_add_nonempty fm f objs) P.
 
-    Module ObjectSet := FSetWeakList.Make(AODec).
-    Module AOMap := FMapWeakList.Make(AODec).
+  Definition upd_points_to (P : PointsTo) (targets : ObjectSet.t) (f : FieldKey)
+                           (new_objs : ObjectSet.t) : PointsTo :=
+    if Nat.eqb (ObjectSet.cardinal targets) 1 then
+      match ObjectSet.choose targets with
+      | Some tgt => points_to_update P tgt f new_objs
+      | None => P
+      end
+    else
+      ObjectSet.fold (fun tgt acc =>
+        let old := points_to_lookup acc tgt f in
+        points_to_update acc tgt f (ObjectSet.union old new_objs)
+      ) targets P.
 
-    Module FKDec <: DecidableType.
-      Definition t := FieldKey.
-      Definition eq := @eq t.
-      Definition eq_refl := @eq_refl t.
-      Definition eq_sym := @eq_sym t.
-      Definition eq_trans := @eq_trans t.
-      Definition eq_dec : forall x y : t, {x = y} + {x <> y}.
-      Proof. decide equality; try apply Nat.eq_dec; try apply String.string_dec. Defined.
-    End FKDec.
+  Definition index_lookup (P : PointsTo) (objs : ObjectSet.t) (idx : nat) : ObjectSet.t :=
+    ObjectSet.fold (fun o acc =>
+      let from_pos  := points_to_lookup P o (FKPos idx) in
+      let from_wild := points_to_lookup P o wildcard in
+      ObjectSet.union acc (ObjectSet.union from_pos from_wild)
+    ) objs ObjectSet.empty.
 
-    Module FieldMap := FMapWeakList.Make(FKDec).
+  (* Type ops *)
+  Definition type_lookup (T : TypeMap) (o : AbstractObject.t) : TypeExpr :=
+    match AOMap.find o T with | Some ty => ty | None => type_bot end.
+  Definition type_update (T : TypeMap) (o : AbstractObject.t) (ty : TypeExpr) : TypeMap :=
+    AOMap.add o (type_join (type_lookup T o) ty) T.
+  Definition type_update_set (T : TypeMap) (objs : ObjectSet.t) (ty : TypeExpr) : TypeMap :=
+    ObjectSet.fold (fun o acc => type_update acc o ty) objs T.
+  Definition get_types (T : TypeMap) (objs : ObjectSet.t) : TypeExpr :=
+    ObjectSet.fold (fun o acc => type_join acc (type_lookup T o)) objs type_bot.
 
-    Definition PointsTo := AOMap.t (FieldMap.t ObjectSet.t).
-    Definition TypeMap  := AOMap.t TS.TypeExpr.
-    Definition DirtyMap := AOMap.t (FieldMap.t bool).
-    Definition StackEnv := StackVar -> ObjectSet.t.
-    Definition ProgramPoint := (nat * nat)%type.
+  (* Dirty *)
+  Definition mark_dirty (D : DirtyMap) (o : AbstractObject.t) (f : FieldKey) : DirtyMap :=
+    let fm := match AOMap.find o D with | Some fm => fm | None => FieldMap.empty _ end in
+    AOMap.add o (FieldMap.add f true fm) D.
+  Definition mark_dirty_set (D : DirtyMap) (objs : ObjectSet.t) (f : FieldKey) : DirtyMap :=
+    ObjectSet.fold (fun o acc => mark_dirty acc o f) objs D.
 
-    (* ===== Field Key Helpers ===== *)
-    Definition wildcard    : FieldKey := FKName "*".
-    Definition self_field  : FieldKey := FKName "self".
-    Definition func_field  : FieldKey := FKName "__func__".
-    Definition args_field  : FieldKey := FKName "args".
-    Definition kwargs_field: FieldKey := FKName "kwargs".
+  (* Stack *)
+  Definition stack_lookup (S : StackEnv) (v : StackVar) : ObjectSet.t := S v.
+  Definition stack_update (S : StackEnv) (v : StackVar) (objs : ObjectSet.t) : StackEnv :=
+    fun v' => if Nat.eqb v v' then objs else S v'.
 
-    Definition is_star (k:FieldKey) : bool :=
-      match k with | FKName s => String.eqb s "*" | _ => false end.
+  (* Unified State *)
+  Record State := {
+    st_points_to : PointsTo;
+    st_types     : TypeMap;
+    st_dirty     : DirtyMap;
+    st_stack     : StackEnv
+  }.
 
-    Definition field_matches (k1 k2 : FieldKey) : bool :=
-      if orb (is_star k1) (is_star k2) then true else
-      match k1, k2 with
-      | FKPos n1,  FKPos n2  => Nat.eqb n1 n2
-      | FKName s1, FKName s2 => String.eqb s1 s2
-      | FKBoth n1 s1, FKBoth n2 s2 => Nat.eqb n1 n2 && String.eqb s1 s2
-      | FKPos n,   FKBoth n' _ | FKBoth n' _, FKPos n   => Nat.eqb n n'
-      | FKName s,  FKBoth _ s' | FKBoth _ s', FKName s  => String.eqb s s'
-      | _, _ => false
-      end.
+  Definition empty_state : State := {|
+    st_points_to := empty_points_to;
+    st_types     := empty_type_map;
+    st_dirty     := empty_dirty_map;
+    st_stack     := empty_stack
+  |}.
 
-    (* ===== Empty/Initial Values ===== *)
-    Definition empty_points_to : PointsTo := AOMap.empty _.
-    Definition empty_type_map  : TypeMap  := AOMap.empty _.
-    Definition empty_dirty_map : DirtyMap := AOMap.empty _.
-    Definition empty_stack     : StackEnv := fun _ => ObjectSet.empty.
+  Definition with_points (s : State) (P : PointsTo) : State :=
+    {| st_points_to := P; st_types := st_types s; st_dirty := st_dirty s; st_stack := st_stack s |}.
+  Definition with_types  (s : State) (T : TypeMap)  : State :=
+    {| st_points_to := st_points_to s; st_types := T; st_dirty := st_dirty s; st_stack := st_stack s |}.
+  Definition with_dirty  (s : State) (D : DirtyMap) : State :=
+    {| st_points_to := st_points_to s; st_types := st_types s; st_dirty := D; st_stack := st_stack s |}.
+  Definition with_stack  (s : State) (S : StackEnv) : State :=
+    {| st_points_to := st_points_to s; st_types := st_types s; st_dirty := st_dirty s; st_stack := S |}.
+  Definition with_pts_ty_dirty (s:State) (P:PointsTo) (T:TypeMap) (D:DirtyMap) : State :=
+    {| st_points_to := P; st_types := T; st_dirty := D; st_stack := st_stack s |}.
 
-    (* ===== Helpers for immutables ===== *)
-    Definition immutable_const (c : ConstV) : ObjectSet.t :=
-      ObjectSet.singleton (ImmConst c).
-    Definition immutable_type (ty : TypeExpr) : ObjectSet.t :=
-      ObjectSet.singleton (ImmType (get_type_hash ty)).
+  (* Location & env helpers *)
+  Definition alloc_site (pp : ProgramPoint) : AbstractObject.t :=
+    let '(b,i) := pp in AbstractObject.Location b i.
 
-    (* Keep FieldMap sparse *)
-    Definition fm_add_nonempty (fm : FieldMap.t ObjectSet.t)
-                               (k : FieldKey) (objs : ObjectSet.t)
-      : FieldMap.t ObjectSet.t :=
-      if ObjectSet.is_empty objs then FieldMap.remove k fm
-      else FieldMap.add k objs fm.
+  Definition get_local  (P : PointsTo) (name : string) : ObjectSet.t :=
+    points_to_lookup P AbstractObject.Locals (FKName name).
+  Definition set_local  (P : PointsTo) (name : string) (objs : ObjectSet.t) : PointsTo :=
+    upd_points_to P (ObjectSet.singleton AbstractObject.Locals) (FKName name) objs.
+  Definition get_global (P : PointsTo) (name : string) : ObjectSet.t :=
+    points_to_lookup P AbstractObject.Globals (FKName name).
 
-    (* ===== Points-to ops ===== *)
-    Definition points_to_lookup (P : PointsTo) (o : AbstractObject.t) (f : FieldKey) : ObjectSet.t :=
-      match AOMap.find o P with
-      | Some fm =>
-          FieldMap.fold (fun k objs acc =>
-            if orb (field_matches k f) (field_matches f k)
-            then ObjectSet.union acc objs
-            else acc) fm ObjectSet.empty
-      | None => ObjectSet.empty
-      end.
+  (* Attribute evaluation *)
+  Definition eval_const (c : ConstV) : (ObjectSet.t * TypeExpr) :=
+    let ty := literal_type c in (immutable_const c, ty).
 
-    Definition points_to_update (P : PointsTo) (o : AbstractObject.t) (f : FieldKey)
-                                (objs : ObjectSet.t) : PointsTo :=
-      let fm := match AOMap.find o P with
-                | Some fm => fm | None => FieldMap.empty _
-                end in
-      AOMap.add o (fm_add_nonempty fm f objs) P.
-
-    Definition upd_points_to (P : PointsTo) (targets : ObjectSet.t) (f : FieldKey)
-                             (new_objs : ObjectSet.t) : PointsTo :=
-      if Nat.eqb (ObjectSet.cardinal targets) 1 then
-        match ObjectSet.choose targets with
-        | Some tgt => points_to_update P tgt f new_objs
-        | None => P
-        end
+  Definition eval_attribute (st : State) (var_objs : ObjectSet.t)
+                            (attr : string) (pp : ProgramPoint)
+    : (State * ObjectSet.t * TypeExpr) :=
+    let var_type    := get_types (st_types st) var_objs in
+    let attr_type   := subscr var_type attr in
+    let result_type := if is_property attr_type then get_return attr_type else attr_type in
+    let res :=
+      if type_is_immutable result_type then
+        (st, immutable_type result_type)
+      else if is_bound_method attr_type then
+        let bm := alloc_site pp in
+        let func_objs :=
+          ObjectSet.fold (fun o acc =>
+            ObjectSet.union acc (points_to_lookup (st_points_to st) o (FKName attr)))
+            var_objs ObjectSet.empty in
+        let P0 := upd_points_to (st_points_to st) (ObjectSet.singleton bm) self_field var_objs in
+        let P1 := upd_points_to P0 (ObjectSet.singleton bm) func_field func_objs in
+        let T' := type_update (st_types st) bm attr_type in
+        (with_pts_ty_dirty st P1 T' (st_dirty st), ObjectSet.singleton bm)
+      else if andb (any_new attr_type) (all_new attr_type) then
+        let new_obj := alloc_site pp in
+        let T' := type_update (st_types st) new_obj result_type in
+        (with_types st T', ObjectSet.singleton new_obj)
       else
-        ObjectSet.fold (fun tgt acc =>
-          let old := points_to_lookup acc tgt f in
-          points_to_update acc tgt f (ObjectSet.union old new_objs)
-        ) targets P.
-
-    Definition index_lookup (P : PointsTo) (objs : ObjectSet.t) (idx : nat) : ObjectSet.t :=
-      ObjectSet.fold (fun o acc =>
-        let from_pos  := points_to_lookup P o (FKPos idx) in
-        let from_wild := points_to_lookup P o wildcard in
-        ObjectSet.union acc (ObjectSet.union from_pos from_wild)
-      ) objs ObjectSet.empty.
-
-    (* ===== Type ops ===== *)
-    Definition type_lookup (T : TypeMap) (o : AbstractObject.t) : TypeExpr :=
-      match AOMap.find o T with | Some ty => ty | None => type_bot end.
-    Definition type_update (T : TypeMap) (o : AbstractObject.t) (ty : TypeExpr) : TypeMap :=
-      AOMap.add o (type_join (type_lookup T o) ty) T.
-    Definition type_update_set (T : TypeMap) (objs : ObjectSet.t) (ty : TypeExpr) : TypeMap :=
-      ObjectSet.fold (fun o acc => type_update acc o ty) objs T.
-    Definition get_types (T : TypeMap) (objs : ObjectSet.t) : TypeExpr :=
-      ObjectSet.fold (fun o acc => type_join acc (type_lookup T o)) objs type_bot.
-
-    (* ===== Dirty ===== *)
-    Definition mark_dirty (D : DirtyMap) (o : AbstractObject.t) (f : FieldKey) : DirtyMap :=
-      let fm := match AOMap.find o D with | Some fm => fm | None => FieldMap.empty _ end in
-      AOMap.add o (FieldMap.add f true fm) D.
-    Definition mark_dirty_set (D : DirtyMap) (objs : ObjectSet.t) (f : FieldKey) : DirtyMap :=
-      ObjectSet.fold (fun o acc => mark_dirty acc o f) objs D.
-
-    (* ===== Stack ===== *)
-    Definition stack_lookup (S : StackEnv) (v : StackVar) : ObjectSet.t := S v.
-    Definition stack_update (S : StackEnv) (v : StackVar) (objs : ObjectSet.t) : StackEnv :=
-      fun v' => if Nat.eqb v v' then objs else S v'.
-
-    (* ===== Unified State ===== *)
-    Record State := {
-      st_points_to : PointsTo;
-      st_types     : TypeMap;
-      st_dirty     : DirtyMap;
-      st_stack     : StackEnv
-    }.
-
-    Definition empty_state : State := {|
-      st_points_to := empty_points_to;
-      st_types     := empty_type_map;
-      st_dirty     := empty_dirty_map;
-      st_stack     := empty_stack
-    |}.
-
-    Definition with_points (s : State) (P : PointsTo) : State :=
-      {| st_points_to := P; st_types := st_types s; st_dirty := st_dirty s; st_stack := st_stack s |}.
-    Definition with_types  (s : State) (T : TypeMap)  : State :=
-      {| st_points_to := st_points_to s; st_types := T; st_dirty := st_dirty s; st_stack := st_stack s |}.
-    Definition with_dirty  (s : State) (D : DirtyMap) : State :=
-      {| st_points_to := st_points_to s; st_types := st_types s; st_dirty := D; st_stack := st_stack s |}.
-    Definition with_stack  (s : State) (S : StackEnv) : State :=
-      {| st_points_to := st_points_to s; st_types := st_types s; st_dirty := st_dirty s; st_stack := S |}.
-    Definition with_pts_ty_dirty (s:State) (P:PointsTo) (T:TypeMap) (D:DirtyMap) : State :=
-      {| st_points_to := P; st_types := T; st_dirty := D; st_stack := st_stack s |}.
-
-    (* ===== Location & env helpers ===== *)
-    Definition alloc_site (pp : ProgramPoint) : AbstractObject.t :=
-      let '(b,i) := pp in Location b i.
-
-    Definition get_local  (P : PointsTo) (name : string) : ObjectSet.t :=
-      points_to_lookup P Locals (FKName name).
-    Definition set_local  (P : PointsTo) (name : string) (objs : ObjectSet.t) : PointsTo :=
-      upd_points_to P (ObjectSet.singleton Locals) (FKName name) objs.
-    Definition get_global (P : PointsTo) (name : string) : ObjectSet.t :=
-      points_to_lookup P Globals (FKName name).
-
-    (* ===== Attribute evaluation ===== *)
-    Definition eval_const (c : ConstV) : (ObjectSet.t * TypeExpr) :=
-      let ty := literal_type c in (immutable_const c, ty).
-
-    Definition eval_attribute (st : State) (var_objs : ObjectSet.t)
-                              (attr : string) (pp : ProgramPoint)
-      : (State * ObjectSet.t * TypeExpr) :=
-      let var_type    := get_types (st_types st) var_objs in
-      let attr_type   := subscr var_type attr in
-      let result_type := if is_property attr_type then get_return attr_type else attr_type in
-      let res :=
-        if type_is_immutable result_type then
-          (st, immutable_type result_type)
-        else if is_bound_method attr_type then
-          let bm := alloc_site pp in
-          let func_objs :=
-            ObjectSet.fold (fun o acc =>
-              ObjectSet.union acc (points_to_lookup (st_points_to st) o (FKName attr)))
-              var_objs ObjectSet.empty in
-          let P0 := upd_points_to (st_points_to st) (ObjectSet.singleton bm) self_field var_objs in
-          let P1 := upd_points_to P0 (ObjectSet.singleton bm) func_field func_objs in
-          let T' := type_update (st_types st) bm attr_type in
-          (with_pts_ty_dirty st P1 T' (st_dirty st), ObjectSet.singleton bm)
-        else if andb (any_new attr_type) (all_new attr_type) then
+        let field_objs :=
+          ObjectSet.fold (fun o acc =>
+            ObjectSet.union acc (points_to_lookup (st_points_to st) o (FKName attr)))
+            var_objs ObjectSet.empty in
+        if any_new attr_type then
           let new_obj := alloc_site pp in
           let T' := type_update (st_types st) new_obj result_type in
-          (with_types st T', ObjectSet.singleton new_obj)
-        else
-          let field_objs :=
-            ObjectSet.fold (fun o acc =>
-              ObjectSet.union acc (points_to_lookup (st_points_to st) o (FKName attr)))
-              var_objs ObjectSet.empty in
-          if any_new attr_type then
-            let new_obj := alloc_site pp in
-            let T' := type_update (st_types st) new_obj result_type in
-            (with_types st T', ObjectSet.union field_objs (ObjectSet.singleton new_obj))
-          else (st, field_objs)
-      in
-      let '(st', base_objs) := res in
-      let result_objs :=
-        if type_is_immutable result_type
-        then ObjectSet.union base_objs (immutable_type result_type)
-        else base_objs in
-      (st', result_objs, result_type).
+          (with_types st T', ObjectSet.union field_objs (ObjectSet.singleton new_obj))
+        else (st, field_objs)
+    in
+    let '(st', base_objs) := res in
+    let result_objs :=
+      if type_is_immutable result_type
+      then ObjectSet.union base_objs (immutable_type result_type)
+      else base_objs in
+    (st', result_objs, result_type).
 
-    (* ===== Dunder evaluation ===== *)
-    Definition eval_dunder (st : State) (e : Dunder) (pp : ProgramPoint)
-      : (State * ObjectSet.t * TypeExpr) :=
-      let T := st_types st in
-      match e with
-      | DUnOp op a =>
-          let a_objs := st_stack st a in
-          let a_ty   := get_types T a_objs in
-          let f_ty   := dunder_lookup (TDUnOp op a_ty) in
-          if type_is_immutable f_ty
-          then (st, immutable_type f_ty, f_ty)
-          else let loc := alloc_site pp in
-               let st' := with_types st (type_update T loc f_ty) in
-               (st', ObjectSet.singleton loc, f_ty)
+  (* Dunder evaluation *)
+  Definition eval_dunder (st : State) (e : Dunder) (pp : ProgramPoint)
+    : (State * ObjectSet.t * TypeExpr) :=
+    let T := st_types st in
+    match e with
+    | DUnOp op a =>
+        let a_objs := st_stack st a in
+        let a_ty   := get_types T a_objs in
+        let f_ty   := dunder_lookup (TDUnOp op a_ty) in
+        if type_is_immutable f_ty
+        then (st, immutable_type f_ty, f_ty)
+        else let loc := alloc_site pp in
+             let st' := with_types st (type_update T loc f_ty) in
+             (st', ObjectSet.singleton loc, f_ty)
 
-      | DBinOp op l r mode =>
-          let l_objs := st_stack st l in
-          let r_objs := st_stack st r in
-          let l_ty   := get_types T l_objs in
-          let r_ty   := get_types T r_objs in
-          let f_ty   := dunder_lookup (TDBinOp op l_ty r_ty mode) in
-          if type_is_immutable f_ty
-          then (st, immutable_type f_ty, f_ty)
-          else let loc := alloc_site pp in
-               let st' := with_types st (type_update T loc f_ty) in
-               (st', ObjectSet.singleton loc, f_ty)
+    | DBinOp op l r mode =>
+        let l_objs := st_stack st l in
+        let r_objs := st_stack st r in
+        let l_ty   := get_types T l_objs in
+        let r_ty   := get_types T r_objs in
+        let f_ty   := dunder_lookup (TDBinOp op l_ty r_ty mode) in
+        if type_is_immutable f_ty
+        then (st, immutable_type f_ty, f_ty)
+        else let loc := alloc_site pp in
+             let st' := with_types st (type_update T loc f_ty) in
+             (st', ObjectSet.singleton loc, f_ty)
 
-      | DCmpOp op l r =>
-          let l_objs := st_stack st l in
-          let r_objs := st_stack st r in
-          let l_ty   := get_types T l_objs in
-          let r_ty   := get_types T r_objs in
-          let f_ty   := dunder_lookup (TDCmpOp op l_ty r_ty) in
-          if type_is_immutable f_ty
-          then (st, immutable_type f_ty, f_ty)
-          else let loc := alloc_site pp in
-               let st' := with_types st (type_update T loc f_ty) in
-               (st', ObjectSet.singleton loc, f_ty)
-      end.
+    | DCmpOp op l r =>
+        let l_objs := st_stack st l in
+        let r_objs := st_stack st r in
+        let l_ty   := get_types T l_objs in
+        let r_ty   := get_types T r_objs in
+        let f_ty   := dunder_lookup (TDCmpOp op l_ty r_ty) in
+        if type_is_immutable f_ty
+        then (st, immutable_type f_ty, f_ty)
+        else let loc := alloc_site pp in
+             let st' := with_types st (type_update T loc f_ty) in
+             (st', ObjectSet.singleton loc, f_ty)
+    end.
 
-    (* ===== Bound-call helpers & joins ===== *)
-    Definition collect_wild_values (P:PointsTo) (containers:ObjectSet.t) : ObjectSet.t :=
-      ObjectSet.fold (fun o acc => ObjectSet.union acc (points_to_lookup P o wildcard))
-                     containers ObjectSet.empty.
-    Definition bound_args_tuples (P:PointsTo) (callee:ObjectSet.t) : ObjectSet.t :=
-      ObjectSet.fold (fun f acc => ObjectSet.union acc (points_to_lookup P f args_field))
-                     callee ObjectSet.empty.
-    Definition bound_kwargs_dicts (P:PointsTo) (callee:ObjectSet.t) : ObjectSet.t :=
-      ObjectSet.fold (fun f acc => ObjectSet.union acc (points_to_lookup P f kwargs_field))
-                     callee ObjectSet.empty.
-    Definition bound_self (P:PointsTo) (callee:ObjectSet.t) : ObjectSet.t :=
-      ObjectSet.fold (fun f acc => ObjectSet.union acc (points_to_lookup P f self_field))
-                     callee ObjectSet.empty.
+  (* Bound-call helpers & joins *)
+  Definition collect_wild_values (P:PointsTo) (containers:ObjectSet.t) : ObjectSet.t :=
+    ObjectSet.fold (fun o acc => ObjectSet.union acc (points_to_lookup P o wildcard))
+                   containers ObjectSet.empty.
+  Definition bound_args_tuples (P:PointsTo) (callee:ObjectSet.t) : ObjectSet.t :=
+    ObjectSet.fold (fun f acc => ObjectSet.union acc (points_to_lookup P f args_field))
+                   callee ObjectSet.empty.
+  Definition bound_kwargs_dicts (P:PointsTo) (callee:ObjectSet.t) : ObjectSet.t :=
+    ObjectSet.fold (fun f acc => ObjectSet.union acc (points_to_lookup P f kwargs_field))
+                   callee ObjectSet.empty.
+  Definition bound_self (P:PointsTo) (callee:ObjectSet.t) : ObjectSet.t :=
+    ObjectSet.fold (fun f acc => ObjectSet.union acc (points_to_lookup P f self_field))
+                   callee ObjectSet.empty.
 
-    Definition join_fieldmaps (fm1 fm2 : FieldMap.t ObjectSet.t) : FieldMap.t ObjectSet.t :=
-      FieldMap.fold (fun k objs acc =>
-        let old := match FieldMap.find k acc with | Some o => o | None => ObjectSet.empty end in
-        fm_add_nonempty acc k (ObjectSet.union old objs)
-      ) fm2 fm1.
-    Definition join_points_to (P1 P2 : PointsTo) : PointsTo :=
-      AOMap.fold (fun o fm acc =>
-        let old := match AOMap.find o acc with | Some fm0 => fm0 | None => FieldMap.empty _ end in
-        AOMap.add o (join_fieldmaps old fm) acc
-      ) P2 P1.
-    Definition join_type_maps (T1 T2 : TypeMap) : TypeMap :=
-      AOMap.fold (fun o ty acc =>
-        let old := match AOMap.find o acc with | Some ty0 => ty0 | None => type_bot end in
-        AOMap.add o (type_join old ty) acc
-      ) T2 T1.
-    Definition join_dirty_field (b1 b2 : bool) : bool := orb b1 b2.
-    Definition join_dirty_maps (D1 D2 : DirtyMap) : DirtyMap :=
-      AOMap.fold (fun o fm2 acc =>
-        let fm1 := match AOMap.find o acc with | Some fm => fm | None => FieldMap.empty _ end in
-        let fm' :=
-          FieldMap.fold (fun k b accfm =>
-            let old := match FieldMap.find k accfm with | Some bb => bb | None => false end in
-            FieldMap.add k (join_dirty_field old b) accfm
-          ) fm2 fm1
-        in AOMap.add o fm' acc
-      ) D2 D1.
-    Definition join_stack (S1 S2 : StackEnv) : StackEnv :=
-      fun v => ObjectSet.union (S1 v) (S2 v).
-    Definition join_state (s1 s2 : State) : State :=
-      {| st_points_to := join_points_to (st_points_to s1) (st_points_to s2);
-         st_types     := join_type_maps (st_types s1)     (st_types s2);
-         st_dirty     := join_dirty_maps (st_dirty s1)    (st_dirty s2);
-         st_stack     := join_stack     (st_stack s1)     (st_stack s2) |}.
-         
-    (* Evaluate ILookupOverload: resolve a static callable from func + (args, kwargs). *)
-    Definition eval_lookup_overload
-      (st : State) (func_sv args_sv kwargs_sv : StackVar) (pp : ProgramPoint)
-      : (State * ObjectSet.t * TypeExpr) :=
-      let P := st_points_to st in
-      let T := st_types     st in
+  Definition join_fieldmaps (fm1 fm2 : FieldMap.t ObjectSet.t) : FieldMap.t ObjectSet.t :=
+    FieldMap.fold (fun k objs acc =>
+      let old := match FieldMap.find k acc with | Some o => o | None => ObjectSet.empty end in
+      fm_add_nonempty acc k (ObjectSet.union old objs)
+    ) fm2 fm1.
+  Definition join_points_to (P1 P2 : PointsTo) : PointsTo :=
+    AOMap.fold (fun o fm acc =>
+      let old := match AOMap.find o acc with | Some fm0 => fm0 | None => FieldMap.empty _ end in
+      AOMap.add o (join_fieldmaps old fm) acc
+    ) P2 P1.
+  Definition join_type_maps (T1 T2 : TypeMap) : TypeMap :=
+    AOMap.fold (fun o ty acc =>
+      let old := match AOMap.find o acc with | Some ty0 => ty0 | None => type_bot end in
+      AOMap.add o (type_join old ty) acc
+    ) T2 T1.
+  Definition join_dirty_field (b1 b2 : bool) : bool := orb b1 b2.
+  Definition join_dirty_maps (D1 D2 : DirtyMap) : DirtyMap :=
+    AOMap.fold (fun o fm2 acc =>
+      let fm1 := match AOMap.find o acc with | Some fm => fm | None => FieldMap.empty _ end in
+      let fm' :=
+        FieldMap.fold (fun k b accfm =>
+          let old := match FieldMap.find k accfm with | Some bb => bb | None => false end in
+          FieldMap.add k (join_dirty_field old b) accfm
+        ) fm2 fm1
+      in AOMap.add o fm' acc
+    ) D2 D1.
+  Definition join_stack (S1 S2 : StackEnv) : StackEnv :=
+    fun v => ObjectSet.union (S1 v) (S2 v).
+  Definition join_state (s1 s2 : State) : State :=
+    {| st_points_to := join_points_to (st_points_to s1) (st_points_to s2);
+       st_types     := join_type_maps (st_types s1)     (st_types s2);
+       st_dirty     := join_dirty_maps (st_dirty s1)    (st_dirty s2);
+       st_stack     := join_stack     (st_stack s1)     (st_stack s2) |}.
+       
+  (* Evaluate ILookupOverload *)
+  Definition eval_lookup_overload
+    (st : State) (func_sv args_sv kwargs_sv : StackVar) (pp : ProgramPoint)
+    : (State * ObjectSet.t * TypeExpr) :=
+    let P := st_points_to st in
+    let T := st_types     st in
+  
+    let func_objs   := stack_lookup (st_stack st) func_sv in
+    let args_objs   := stack_lookup (st_stack st) args_sv in
+    let kwargs_objs := stack_lookup (st_stack st) kwargs_sv in
+  
+    let pos_vals := collect_wild_values P args_objs in
+    let kw_vals  := collect_wild_values P kwargs_objs in
+    let arg_types := [ type_join (get_types T pos_vals) (get_types T kw_vals) ] in
+  
+    let func_ty   := get_types T func_objs in
+    let resolved  := partial func_ty arg_types in
+  
+    let res_objs :=
+      if type_is_immutable resolved
+      then immutable_type resolved
+      else ObjectSet.singleton (alloc_site pp) in
+  
+    let st' :=
+      if type_is_immutable resolved
+      then st
+      else with_types st (type_update T (alloc_site pp) resolved) in
+  
+    (st', res_objs, resolved).
+  
+  (* Calls & transfers *)
+  Definition eval_call_single (st : State) (callee : AbstractObject.t) (pp : ProgramPoint)
+    : (State * ObjectSet.t * TypeExpr) :=
+    let P := st_points_to st in
+    let T := st_types st in
+    let callee_set := ObjectSet.singleton callee in
+    let args_tups := bound_args_tuples P callee_set in
+    let kwargs_ds := bound_kwargs_dicts P callee_set in
+    let self_objs := bound_self P callee_set in
+    let pos_vals := collect_wild_values P args_tups in
+    let kw_vals  := collect_wild_values P kwargs_ds in
+    let arg_types := [ type_join (get_types T pos_vals) (get_types T kw_vals) ] in
+    let func_ty   := type_lookup T callee in
+    let applied   := partial func_ty arg_types in
+    let effect    := get_side_effect applied in
+    let ret_ty    := get_return applied in
+    let res_objs :=
+      if type_is_immutable ret_ty then immutable_type ret_ty
+      else if se_new effect then ObjectSet.singleton (alloc_site pp)
+      else if se_points_to_args effect then ObjectSet.union pos_vals kw_vals
+      else ObjectSet.empty in
+    let st' :=
+      match se_update effect with
+      | Some up_ty =>
+          let T' := ObjectSet.fold (fun o acc => type_update acc o up_ty) self_objs T in
+          let D' := mark_dirty_set (st_dirty st) self_objs wildcard in
+          let P' :=
+            match se_update_indices effect with
+            | [] => P
+            | idxs =>
+                List.fold_left (fun acc idx =>
+                   let param_objs := index_lookup P args_tups idx in
+                   upd_points_to acc self_objs wildcard param_objs
+                ) idxs P
+            end in
+          with_pts_ty_dirty st P' T' D'
+      | None => st
+      end in
+    let st'' :=
+      if se_new effect then
+        let T'' := type_update (st_types st') (alloc_site pp) ret_ty in
+        with_types st' T''
+      else st' in
+    let st''' :=
+      if andb (se_new effect) (se_points_to_args effect) then
+        let ali := ObjectSet.union pos_vals kw_vals in
+        let P'' := upd_points_to (st_points_to st'') (ObjectSet.singleton (alloc_site pp)) wildcard ali in
+        with_points st'' P''
+      else st'' in
+    (st''', res_objs, ret_ty).
+
+  Definition eval_call (st : State) (func_objs : ObjectSet.t) (pp : ProgramPoint)
+    : (State * ObjectSet.t * TypeExpr) :=
+    ObjectSet.fold
+      (fun f acc =>
+         let '(acc_st, acc_objs, acc_ty) := acc in
+         let '(one_st, one_objs, one_ty) := eval_call_single acc_st f pp in
+         (one_st, ObjectSet.union acc_objs one_objs, type_join acc_ty one_ty))
+      func_objs
+      (st, ObjectSet.empty, type_bot).
+
+  (* Transfer functions - all the rest remain the same *)
+  Definition transfer_load_const (st : State) (dst : StackVar) (c : ConstV) : State :=
+    let (objs, ty) := eval_const c in
+    let T' := type_update_set (st_types st) objs ty in
+    let st' := with_types st T' in
+    with_stack st' (stack_update (st_stack st) dst objs).
+
+  Definition transfer_load_local (st : State) (dst : StackVar) (name : string) : State :=
+    let objs := get_local (st_points_to st) name in
+    with_stack st (stack_update (st_stack st) dst objs).
+
+  Definition transfer_load_global (st : State) (dst : StackVar) (name : string) : State :=
+    let objs := get_global (st_points_to st) name in
+    with_stack st (stack_update (st_stack st) dst objs).
+
+  Definition transfer_set_local (st : State) (name : string) (src : StackVar) : State :=
+    let objs := stack_lookup (st_stack st) src in
+    let P' := set_local (st_points_to st) name objs in
+    with_points st P'.
+
+  Definition transfer_get_attr (st : State) (dst : StackVar) (obj : StackVar)
+                               (attr : string) (pp : ProgramPoint) : State :=
+    let obj_set := stack_lookup (st_stack st) obj in
+    let (st', result_objs, result_type) := eval_attribute st obj_set attr pp in
+    let T' := type_update_set (st_types st') result_objs result_type in
+    let st'' := with_types st' T' in
+    with_stack st'' (stack_update (st_stack st'') dst result_objs).
+
+  Definition transfer_set_attr (st : State) (obj : StackVar) (attr : string)
+                               (val : StackVar) : State :=
+    let targets := stack_lookup (st_stack st) obj in
+    let values  := stack_lookup (st_stack st) val in
+    let P' := upd_points_to (st_points_to st) targets (FKName attr) values in
+    let D' := mark_dirty_set (st_dirty st) targets (FKName attr) in
+    with_pts_ty_dirty st P' (st_types st) D'.
+
+  Definition transfer_construct_tuple (st : State) (dst : StackVar) (elems : list StackVar)
+                                     (pp : ProgramPoint) : State :=
+    let tup := alloc_site pp in
+    let indexed_elems := List.combine (List.seq 0 (List.length elems)) elems in
+    let P' := List.fold_left (fun acc pair =>
+      let (idx, elem) := pair in
+      let elem_objs := stack_lookup (st_stack st) elem in
+      let P1 := upd_points_to acc (ObjectSet.singleton tup) (FKPos idx) elem_objs in
+      upd_points_to P1 (ObjectSet.singleton tup) wildcard elem_objs
+    ) indexed_elems (st_points_to st) in
+    let T' := type_update (st_types st) tup (get_return make_tuple_constructor) in
+    let st' := with_pts_ty_dirty st P' T' (st_dirty st) in
+    with_stack st' (stack_update (st_stack st') dst (ObjectSet.singleton tup)).
+
+  Definition transfer_construct_dict (st : State) (dst : StackVar)
+                                     (pairs : list (StackVar * StackVar))
+                                     (pp : ProgramPoint) : State :=
+    let dict := alloc_site pp in
+    let P' := List.fold_left (fun acc pair =>
+      let (key_var, val_var) := pair in
+      let key_objs := stack_lookup (st_stack st) key_var in
+      let val_objs := stack_lookup (st_stack st) val_var in
+      let P0 := upd_points_to acc (ObjectSet.singleton dict) wildcard val_objs in
+      match ObjectSet.choose key_objs with
+      | Some (AbstractObject.ImmConst (KString s)) =>
+          if Nat.eqb (ObjectSet.cardinal key_objs) 1
+          then upd_points_to P0 (ObjectSet.singleton dict) (FKName s) val_objs
+          else P0
+      | _ => P0
+      end
+    ) pairs (st_points_to st) in
+    let T' := type_update (st_types st) dict (get_return make_dict_constructor) in
+    let st' := with_pts_ty_dirty st P' T' (st_dirty st) in
+    with_stack st' (stack_update (st_stack st') dst (ObjectSet.singleton dict)).
+
+  Definition transfer_bind (st : State) (dst func_var args_var kwargs_var : StackVar)
+                           (pp : ProgramPoint) : State :=
+    let bound      := alloc_site pp in
+    let func_objs  := stack_lookup (st_stack st) func_var in
+    let args_objs  := stack_lookup (st_stack st) args_var in
+    let kwargs_objs:= stack_lookup (st_stack st) kwargs_var in
+    let P1 := upd_points_to (st_points_to st) (ObjectSet.singleton bound) func_field  func_objs in
+    let P2 := upd_points_to P1                 (ObjectSet.singleton bound) args_field  args_objs in
+    let P3 := upd_points_to P2                 (ObjectSet.singleton bound) kwargs_field kwargs_objs in
+    let self_objs := index_lookup P3 args_objs 0 in
+    let P4 := if ObjectSet.is_empty self_objs then P3
+              else upd_points_to P3 (ObjectSet.singleton bound) self_field self_objs in
+    let T' := type_update (st_types st) bound (get_types (st_types st) func_objs) in
+    let st' := with_pts_ty_dirty st P4 T' (st_dirty st) in
+    with_stack st' (stack_update (st_stack st') dst (ObjectSet.singleton bound)).
+
+  Definition transfer_unpack (st : State) (dsts : list StackVar) (src : StackVar) : State :=
+    let src_objs := stack_lookup (st_stack st) src in
+    let indexed_dsts := List.combine (List.seq 0 (List.length dsts)) dsts in
+    let S' := List.fold_left (fun acc pair =>
+      let (idx, dst) := pair in
+      let objs := index_lookup (st_points_to st) src_objs idx in
+      stack_update acc dst objs
+    ) indexed_dsts (st_stack st) in
+    with_stack st S'.
     
-      (* Fetch objects *)
-      let func_objs   := stack_lookup (st_stack st) func_sv in
-      let args_objs   := stack_lookup (st_stack st) args_sv in
-      let kwargs_objs := stack_lookup (st_stack st) kwargs_sv in
+  Definition transfer_lookup_dunder
+    (st : State) (dst : StackVar) (expr : Dunder) (pp : ProgramPoint) : State :=
+    let (st', objs, ty) := eval_dunder st expr pp in
+    let T' := type_update_set (st_types st') objs ty in
+    let st'' := with_types st' T' in
+    with_stack st'' (stack_update (st_stack st'') dst objs). 
     
-      (* Build coarse argument-type summary from tuple/dict wildcards *)
-      let pos_vals := collect_wild_values P args_objs in
-      let kw_vals  := collect_wild_values P kwargs_objs in
-      let arg_types := [ type_join (get_types T pos_vals) (get_types T kw_vals) ] in
+  Definition transfer_lookup_overload
+    (st : State) (dst func_sv args_sv kwargs_sv : StackVar) (pp : ProgramPoint) : State :=
+    let (st', objs, ty) := eval_lookup_overload st func_sv args_sv kwargs_sv pp in
+    let T' := type_update_set (st_types st') objs ty in
+    let st'' := with_types st' T' in
+    with_stack st'' (stack_update (st_stack st'') dst objs).
     
-      (* Resolve overload/type via TS.partial *)
-      let func_ty   := get_types T func_objs in
-      let resolved  := partial func_ty arg_types in
-    
-      (* Materialize the function value *)
-      let res_objs :=
-        if type_is_immutable resolved
-        then immutable_type resolved
-        else ObjectSet.singleton (alloc_site pp) in
-    
-      (* If we allocated, attach the type to that alloc site *)
-      let st' :=
-        if type_is_immutable resolved
-        then st
-        else with_types st (type_update T (alloc_site pp) resolved) in
-    
-      (st', res_objs, resolved).
-    
-    (* ===== Calls & transfers ===== *)
-    Definition eval_call_single (st : State) (callee : AbstractObject.t) (pp : ProgramPoint)
-      : (State * ObjectSet.t * TypeExpr) :=
-      let P := st_points_to st in
-      let T := st_types st in
-      let callee_set := ObjectSet.singleton callee in
-      let args_tups := bound_args_tuples P callee_set in
-      let kwargs_ds := bound_kwargs_dicts P callee_set in
-      let self_objs := bound_self P callee_set in
-      let pos_vals := collect_wild_values P args_tups in
-      let kw_vals  := collect_wild_values P kwargs_ds in
-      let arg_types := [ type_join (get_types T pos_vals) (get_types T kw_vals) ] in
-      let func_ty   := type_lookup T callee in
-      let applied   := partial func_ty arg_types in
-      let effect    := get_side_effect applied in
-      let ret_ty    := get_return applied in
-      let res_objs :=
-        if type_is_immutable ret_ty then immutable_type ret_ty
-        else if se_new effect then ObjectSet.singleton (alloc_site pp)
-        else if se_points_to_args effect then ObjectSet.union pos_vals kw_vals
-        else ObjectSet.empty in
-      let st' :=
-        match se_update effect with
-        | Some up_ty =>
-            let T' := ObjectSet.fold (fun o acc => type_update acc o up_ty) self_objs T in
-            let D' := mark_dirty_set (st_dirty st) self_objs wildcard in
-            let P' :=
-              match se_update_indices effect with
-              | [] => P
-              | idxs =>
-                  List.fold_left (fun acc idx =>
-                     let param_objs := index_lookup P args_tups idx in
-                     upd_points_to acc self_objs wildcard param_objs
-                  ) idxs P
-              end in
-            with_pts_ty_dirty st P' T' D'
-        | None => st
-        end in
-      let st'' :=
-        if se_new effect then
-          let T'' := type_update (st_types st') (alloc_site pp) ret_ty in
-          with_types st' T''
-        else st' in
-      let st''' :=
-        if andb (se_new effect) (se_points_to_args effect) then
-          let ali := ObjectSet.union pos_vals kw_vals in
-          let P'' := upd_points_to (st_points_to st'') (ObjectSet.singleton (alloc_site pp)) wildcard ali in
-          with_points st'' P''
-        else st'' in
-      (st''', res_objs, ret_ty).
+  Definition transfer_call (st : State) (dst : StackVar) (func : StackVar) (pp : ProgramPoint) : State :=
+    let func_objs := stack_lookup (st_stack st) func in
+    let (st', result_objs, result_type) := eval_call st func_objs pp in
+    let T' := type_update_set (st_types st') result_objs result_type in
+    let st'' := with_types st' T' in
+    with_stack st'' (stack_update (st_stack st'') dst result_objs).
 
-    Definition eval_call (st : State) (func_objs : ObjectSet.t) (pp : ProgramPoint)
-      : (State * ObjectSet.t * TypeExpr) :=
-      ObjectSet.fold
-        (fun f acc =>
-           let '(acc_st, acc_objs, acc_ty) := acc in
-           let '(one_st, one_objs, one_ty) := eval_call_single acc_st f pp in
-           (one_st, ObjectSet.union acc_objs one_objs, type_join acc_ty one_ty))
-        func_objs
-        (st, ObjectSet.empty, type_bot).
-
-    Definition transfer_load_const (st : State) (dst : StackVar) (c : ConstV) : State :=
-      let (objs, ty) := eval_const c in
-      let T' := type_update_set (st_types st) objs ty in
-      let st' := with_types st T' in
-      with_stack st' (stack_update (st_stack st) dst objs).
-
-    Definition transfer_load_local (st : State) (dst : StackVar) (name : string) : State :=
-      let objs := get_local (st_points_to st) name in
-      with_stack st (stack_update (st_stack st) dst objs).
-
-    Definition transfer_load_global (st : State) (dst : StackVar) (name : string) : State :=
-      let objs := get_global (st_points_to st) name in
-      with_stack st (stack_update (st_stack st) dst objs).
-
-    Definition transfer_set_local (st : State) (name : string) (src : StackVar) : State :=
-      let objs := stack_lookup (st_stack st) src in
-      let P' := set_local (st_points_to st) name objs in
-      with_points st P'.
-
-    Definition transfer_get_attr (st : State) (dst : StackVar) (obj : StackVar)
-                                 (attr : string) (pp : ProgramPoint) : State :=
-      let obj_set := stack_lookup (st_stack st) obj in
-      let (st', result_objs, result_type) := eval_attribute st obj_set attr pp in
-      let T' := type_update_set (st_types st') result_objs result_type in
-      let st'' := with_types st' T' in
-      with_stack st'' (stack_update (st_stack st'') dst result_objs).
-
-    Definition transfer_set_attr (st : State) (obj : StackVar) (attr : string)
-                                 (val : StackVar) : State :=
-      let targets := stack_lookup (st_stack st) obj in
-      let values  := stack_lookup (st_stack st) val in
-      let P' := upd_points_to (st_points_to st) targets (FKName attr) values in
-      let D' := mark_dirty_set (st_dirty st) targets (FKName attr) in
-      with_pts_ty_dirty st P' (st_types st) D'.
-
-    Definition transfer_construct_tuple (st : State) (dst : StackVar) (elems : list StackVar)
-                                       (pp : ProgramPoint) : State :=
-      let tup := alloc_site pp in
-      let indexed_elems := List.combine (List.seq 0 (List.length elems)) elems in
-      let P' := List.fold_left (fun acc pair =>
-        let (idx, elem) := pair in
-        let elem_objs := stack_lookup (st_stack st) elem in
-        let P1 := upd_points_to acc (ObjectSet.singleton tup) (FKPos idx) elem_objs in
-        upd_points_to P1 (ObjectSet.singleton tup) wildcard elem_objs
-      ) indexed_elems (st_points_to st) in
-      let T' := type_update (st_types st) tup (get_return make_tuple_constructor) in
-      let st' := with_pts_ty_dirty st P' T' (st_dirty st) in
-      with_stack st' (stack_update (st_stack st') dst (ObjectSet.singleton tup)).
-
-    Definition transfer_construct_dict (st : State) (dst : StackVar)
-                                       (pairs : list (StackVar * StackVar))
-                                       (pp : ProgramPoint) : State :=
-      let dict := alloc_site pp in
-      let P' := List.fold_left (fun acc pair =>
-        let (key_var, val_var) := pair in
-        let key_objs := stack_lookup (st_stack st) key_var in
-        let val_objs := stack_lookup (st_stack st) val_var in
-        let P0 := upd_points_to acc (ObjectSet.singleton dict) wildcard val_objs in
-        match ObjectSet.choose key_objs with
-        | Some (ImmConst (KString s)) =>
-            if Nat.eqb (ObjectSet.cardinal key_objs) 1
-            then upd_points_to P0 (ObjectSet.singleton dict) (FKName s) val_objs
-            else P0
-        | _ => P0
-        end
-      ) pairs (st_points_to st) in
-      let T' := type_update (st_types st) dict (get_return make_dict_constructor) in
-      let st' := with_pts_ty_dirty st P' T' (st_dirty st) in
-      with_stack st' (stack_update (st_stack st') dst (ObjectSet.singleton dict)).
-
-    Definition transfer_bind (st : State) (dst func_var args_var kwargs_var : StackVar)
-                             (pp : ProgramPoint) : State :=
-      let bound      := alloc_site pp in
-      let func_objs  := stack_lookup (st_stack st) func_var in
-      let args_objs  := stack_lookup (st_stack st) args_var in
-      let kwargs_objs:= stack_lookup (st_stack st) kwargs_var in
-      let P1 := upd_points_to (st_points_to st) (ObjectSet.singleton bound) func_field  func_objs in
-      let P2 := upd_points_to P1                 (ObjectSet.singleton bound) args_field  args_objs in
-      let P3 := upd_points_to P2                 (ObjectSet.singleton bound) kwargs_field kwargs_objs in
-      let self_objs := index_lookup P3 args_objs 0 in
-      let P4 := if ObjectSet.is_empty self_objs then P3
-                else upd_points_to P3 (ObjectSet.singleton bound) self_field self_objs in
-      let T' := type_update (st_types st) bound (get_types (st_types st) func_objs) in
-      let st' := with_pts_ty_dirty st P4 T' (st_dirty st) in
-      with_stack st' (stack_update (st_stack st') dst (ObjectSet.singleton bound)).
-
-    Definition transfer_unpack (st : State) (dsts : list StackVar) (src : StackVar) : State :=
-      let src_objs := stack_lookup (st_stack st) src in
-      let indexed_dsts := List.combine (List.seq 0 (List.length dsts)) dsts in
-      let S' := List.fold_left (fun acc pair =>
-        let (idx, dst) := pair in
-        let objs := index_lookup (st_points_to st) src_objs idx in
-        stack_update acc dst objs
-      ) indexed_dsts (st_stack st) in
-      with_stack st S'.
-      
-    Definition transfer_lookup_dunder
-      (st : State) (dst : StackVar) (expr : Dunder) (pp : ProgramPoint) : State :=
-      let (st', objs, ty) := eval_dunder st expr pp in
-      let T' := type_update_set (st_types st') objs ty in
-      let st'' := with_types st' T' in
-      with_stack st'' (stack_update (st_stack st'') dst objs). 
-      
-    Definition transfer_lookup_overload
-      (st : State) (dst func_sv args_sv kwargs_sv : StackVar) (pp : ProgramPoint) : State :=
-      let (st', objs, ty) := eval_lookup_overload st func_sv args_sv kwargs_sv pp in
-      let T' := type_update_set (st_types st') objs ty in
-      let st'' := with_types st' T' in
-      with_stack st'' (stack_update (st_stack st'') dst objs).
-      
-    Definition transfer_call (st : State) (dst : StackVar) (func : StackVar) (pp : ProgramPoint) : State :=
-      let func_objs := stack_lookup (st_stack st) func in
-      let (st', result_objs, result_type) := eval_call st func_objs pp in
-      let T' := type_update_set (st_types st') result_objs result_type in
-      let st'' := with_types st' T' in
-      with_stack st'' (stack_update (st_stack st'') dst result_objs).
-
-    (* Main transfer dispatcher *)
-    Definition transfer (st : State) (instr : Instruction) (pp : ProgramPoint) : State :=
-      match instr with
-      | IMov d s => with_stack st (stack_update (st_stack st) d (stack_lookup (st_stack st) s))
-      | ILoadConst d c => transfer_load_const st d c
-      | ILoadLocal d x => transfer_load_local st d x
-      | ILoadGlobal d x => transfer_load_global st d x
-      | ISetLocal x s => transfer_set_local st x s
-      | IGetAttr d o a => transfer_get_attr st d o a pp
-      | ISetAttr o a v => transfer_set_attr st o a v
-      | IConstructTuple d xs => transfer_construct_tuple st d xs pp
-      | IConstructDict d kvs => transfer_construct_dict st d kvs pp
-      | IBind d f a k => transfer_bind st d f a k pp
-      | IUnpack ds s => transfer_unpack st ds s
-      | ICall d f => transfer_call st d f pp
-      | ILookupDunder d expr => transfer_lookup_dunder st d expr pp
-      | ILookupOverload d f a k => transfer_lookup_overload st d f a k pp
-      | IAssumeValue _ _ => st
-      | IExit => st
-      end.
-
-  End Analysis.
+  (* Main transfer dispatcher *)
+  Definition transfer (st : State) (instr : Instruction) (pp : ProgramPoint) : State :=
+    match instr with
+    | IMov d s => with_stack st (stack_update (st_stack st) d (stack_lookup (st_stack st) s))
+    | ILoadConst d c => transfer_load_const st d c
+    | ILoadLocal d x => transfer_load_local st d x
+    | ILoadGlobal d x => transfer_load_global st d x
+    | ISetLocal x s => transfer_set_local st x s
+    | IGetAttr d o a => transfer_get_attr st d o a pp
+    | ISetAttr o a v => transfer_set_attr st o a v
+    | IConstructTuple d xs => transfer_construct_tuple st d xs pp
+    | IConstructDict d kvs => transfer_construct_dict st d kvs pp
+    | IBind d f a k => transfer_bind st d f a k pp
+    | IUnpack ds s => transfer_unpack st ds s
+    | ICall d f => transfer_call st d f pp
+    | ILookupDunder d expr => transfer_lookup_dunder st d expr pp
+    | ILookupOverload d f a k => transfer_lookup_overload st d f a k pp
+    | IAssumeValue _ _ => st
+    | IExit => st
+    end.
 
 End PointerAnalysis.
